cfrontend/BeePL_typesystem.v
@@ -11,8 +11,15 @@ Inductive type_expr : ty_context -> store_context -> expr -> effect -> type -> P
            get_ty Gamma x.(vname) = Some t ->
            x.(vtype) = t ->
            type_expr Gamma Sigma (Var x) empty_effect t
-| Ty_const : forall Gamma Sigma c t,
-             type_expr Gamma Sigma (Const c t) empty_effect t
+| Ty_constint : forall Gamma Sigma t sz s i,
+                t = (Ptype (Tint sz s)) ->
+                type_expr Gamma Sigma (Const (ConsInt i) t) empty_effect t
+| Ty_constbool : forall Gamma Sigma t b,
+                 t = (Ptype Tbool) ->
+                 type_expr Gamma Sigma (Const (ConsBool b) t) empty_effect t
+| Ty_constunit : forall Gamma Sigma t,
+                t = (Ptype Tunit) ->
+                type_expr Gamma Sigma (Const (ConsUnit) t) empty_effect t
 | Ty_appr : forall Gamma Sigma r e es h bt rt ef efs ts, 
             get_ty Gamma r.(vname) = Some rt ->
             type_expr Gamma Sigma (Var r) empty_effect rt -> 
@@ -36,10 +43,11 @@ Inductive type_expr : ty_context -> store_context -> expr -> effect -> type -> P
 | Ty_prim_uop : forall Gamma Sigma op e ef t,
                 type_expr Gamma Sigma e ef t ->
                 type_expr Gamma Sigma (Prim (Uop op) (e::nil) t) ef t 
-| Ty_prim_bop : forall Gamma Sigma op e ef t e',
+| Ty_prim_bop : forall Gamma Sigma op e ef t tr e',
                 type_expr Gamma Sigma e ef t ->
                 type_expr Gamma Sigma e' ef t ->
-                type_expr Gamma Sigma (Prim (Bop op) (e::e'::nil) t) ef t 
+                eq_type tr (if is_not_comparison op then t else (Ptype Tbool)) ->
+                type_expr Gamma Sigma (Prim (Bop op) (e::e'::nil) tr) ef tr 
 | Ty_bind : forall Gamma Sigma x t e e' t' ef,
             type_expr Gamma Sigma e' ef t' ->
             type_expr (extend_context Gamma x t) Sigma e ef t ->
@@ -65,98 +73,361 @@ with type_exprs : ty_context -> store_context -> list expr -> effect -> list typ
 (**** Supoorting lemmas ****)
 Lemma type_rel_typeof : forall Gamma Sigma e ef t,
 type_expr Gamma Sigma e ef t ->
-typeof_expr e = t.
+typeof_expr e = match e with 
+                | Prim (Bop op) es t => (if (is_not_comparison op) then t else (Ptype Tbool)) 
+                | _ => t
+                end.
 Proof.
 move=> Gamma Sigma e ef t ht; inversion ht; subst; rewrite /typeof_expr /=; auto.
+case: ifP=> //= ho. move: H1. rewrite ho /=. case: t ht=> //= p. by case: p=> //=.
 Qed.
 
 Lemma sem_unary_operation_val_type : forall op v t v', 
 sem_unary_operation op v t = Some v' ->
 typeof_value v t /\ typeof_value v' t.
 Proof.
-(*move=> [].
+move=> [].
 + move=> v t v' hs.
   have ht := extract_type_notbool v t v' hs; subst. split.
   + by case: v hs=> //=.
   case: v' hs=> //=.
   + move=> hs. rewrite /sem_notbool in hs. by case: v hs=> //=.
   + move=> i hs. rewrite /sem_notbool in hs. by case: v hs=> //=.
-  + move=> i hs. rewrite /sem_notbool in hs. by case: v hs=> //=.
-  move=> p hs. rewrite /sem_notbool in hs. by case: v hs=> //=.
+  move=> i hs. rewrite /sem_notbool in hs. by case: v hs=> //=.
 + move=> v t v' hs.
-  have ht := extract_type_notint v t v' hs; subst. case: ht=> //= ht; subst. 
-  + split. 
-    + by case: v hs=> //=.
-    case: v' hs=> //=.
-    + rewrite /sem_notint /=. by case: v=>//=.
+  have [sz [s ht]]:= extract_type_notint v t v' hs; subst. split.
+  + case: v hs=> //=. case: v' hs=> //=.
     + rewrite /sem_notint /=. by case: v=> //=.
-    + rewrite /sem_notint /=. by case: v=> //=.
-    by rewrite /sem_notint /=;case: v=> //=.
-  split=> //=.  
-  + by case: v hs=> //=.
-  case: v' hs=> //=.
-  + rewrite /sem_notint /=. by case: v=>//=.
-  + rewrite /sem_notint /=. case: v=> //= i i'.
-    rewrite /of_int /=. move=> [] //=. case: i=> //=. case: i'=> //=.
-    + rewrite /sem_notint /=. by case: v=> //=.
-    by rewrite /sem_notint /=;case: v=> //=.
-
-  case: 
-  by case: v hs=> //=.
-move=> v t v' hs.
-have ht := extract_type_neg v t v' hs; subst. case: ht=> //= ht; subst. 
+    rewrite /sem_notint /=. by case: v=> //=.
+  rewrite /sem_notint /=. by case: v=> //=.
+move=> v t v' hs. have [sz [s ht]] := extract_type_neg v t v' hs; subst. split.
 + by case: v hs=> //=.
-by case: v hs=> //=.
-Qed.*) Admitted.
+case: v' hs=> //=.
++ rewrite /sem_neg /=. by case: v=> //=.
++ rewrite /sem_neg /=. by case: v=> //=.
+rewrite /sem_neg /=. by case: v=> //=.
+Qed.
 
+Lemma sem_binary_operation_val_type : forall op v1 v2 t v, 
+sem_binary_operation op v1 v2 t t = Some v ->
+typeof_value v (if (is_not_comparison op) then t else (Ptype Tbool)).
+Proof.
+move=> [];rewrite /sem_binary_operation.
++ move=> v1 v2 t v hs. move: hs. rewrite /sem_plus. 
+  case: v1=> //=.
+  + case: v2=> //=. case: t=> //= p. by case: p=> //=.
+  + case: v2=> //=. case: t=> //= p. by case: p=> //= [] s s' i i' [] hv; subst.
+  + case: v2=> //=. case: t=> //= p. by case: p=> //=.
+  case: v2=> //=. case: t=> //= i b. case: b=> //= p. by case: p=> //=.
++ move=> v1 v2 t v hs. move: hs. rewrite /sem_plus. 
+  case: v1=> //=.
+  + case: v2=> //=. case: t=> //= p. by case: p=> //=.
+  + case: v2=> //=. case: t=> //= p. by case: p=> //= [] s s' i i' [] hv; subst.
+  + case: v2=> //=. case: t=> //= p. by case: p=> //=.
+  case: v2=> //=. case: t=> //= i b. case: b=> //= p. by case: p=> //=.
++ move=> v1 v2 t v hs. move: hs. rewrite /sem_plus. 
+  case: v1=> //=.
+  + case: v2=> //=. case: t=> //= p. by case: p=> //=.
+  + case: v2=> //=. case: t=> //= p. by case: p=> //= [] s s' i i' [] hv; subst.
+  + case: v2=> //=. case: t=> //= p. by case: p=> //=.
+  case: v2=> //=. case: t=> //= i b. case: b=> //= p. by case: p=> //=.
++ move=> v1 v2 t v hs. move: hs. rewrite /sem_plus. 
+  case: v1=> //=.
+  + case: v2=> //=. case: t=> //= p. by case: p=> //=.
+  + case: v2=> //=. case: t=> //= p. case: p=> //= i s i1 i2. 
+    case: s=> //=. 
+    + case: i=> //=. by case: ifP=> //= he [] hv; subst.
+    case: i=> //=. by case: ifP=> //= he [] hv; subst.
+  + case: v2=> //=. case: t=> //= p. case: p=> //=.
+    case: v2=> //=. case: t=> //= i b. case: b=> //= p. by case: p=> //=.
++ move=> v1 v2 t v. case: v1=> //=.  
+  + case: v2=> //=. case: t=> //= p. by case: p=> //=.
+    case: v2=> //=. case: t=> //= p. by case: p=> //=.
+  case: v2=> //=. case: t=> //= p. by case:p=> //= b b' [] hv; subst.
+  case: v2=> //=. case: t=> //= i b. case: b=> //= p. by case: p=> //=.
++ move=> v1 v2 t v. case: v1=> //=.  
+  + case: v2=> //=. case: t=> //= p. by case: p=> //=.
+    case: v2=> //=. case: t=> //= p. by case: p=> //=.
+  case: v2=> //=. case: t=> //= p. by case:p=> //= b b' [] hv; subst.
+  case: v2=> //=. case: t=> //= i b. case: b=> //= p. by case: p=> //=.
++ move=> v1 v2 t v. case: v1=> //=.  
+  + case: v2=> //=. case: t=> //= p. by case: p=> //=.
+    case: v2=> //=. case: t=> //= p. by case: p=> //=.
+  case: v2=> //=. case: t=> //= p. by case:p=> //= b b' [] hv; subst.
+  case: v2=> //=. case: t=> //= i b. case: b=> //= p. by case: p=> //=.
++ move=> v1 v2 t v. case: v1=> //=.  
+  + case: v2=> //=. case: t=> //= p. by case: p=> //=.
+    case: v2=> //=. case: t=> //= p. case: p=> //= sz s. case: sz=> //= i i'.
+    by case: ifP=> //= hl [] hv; subst.
+  case: v2=> //=. case: t=> //= p. by case:p=> //= b b' [] hv; subst.
+  case: v2=> //=. case: t=> //= i b. case: b=> //= p. by case: p=> //=.
++ move=> v1 v2 t v. case: v1=> //=.  
+  + case: v2=> //=. case: t=> //= p. by case: p=> //=.
+    case: v2=> //=. case: t=> //= p. case: p=> //= sz s. case: s=> //= i i'.
+    case: sz=> //=. by case: ifP=> //= hl [] hv; subst.
+    case: sz=> //=. by case: ifP=> //= hl [] hv; subst.
+  case: v2=> //=. case: t=> //= p. by case:p=> //= b b' [] hv; subst.
+  case: v2=> //=. case: t=> //= i b. case: b=> //= p. by case: p=> //=.
++ move=> v1 v2 t v. rewrite /is_not_comparison /=. case: v1=> //=.
+  + case: v2=> //=. case: t=> //= p. by case: p=> //= [] [] hv; subst.
+  + case: v2=> //= i i'. case: t=> //= p. case: p=> //= sz s. case: s=> //=.
+    + by case: sz=> //= [] [] hv; subst.
+    + by case: sz=> //= [] [] hv; subst.
+    case: v2=> //= b b'. case: t=> //= p. by case: p=> //= [] [] hv; subst.
+  case: v2=> //=. case: t=> //= i b. case: b=> //= p. by case: p=> //=.
++ move=> v1 v2 t v. rewrite /is_not_comparison /=. case: v1=> //=.
+  + case: v2=> //=. case: t=> //= p. by case: p=> //= [] [] hv; subst.
+  + case: v2=> //= i i'. case: t=> //= p. case: p=> //= sz s. case: s=> //=.
+    + by case: sz=> //= [] [] hv; subst.
+    + by case: sz=> //= [] [] hv; subst.
+    case: v2=> //= b b'. case: t=> //= p. by case: p=> //= [] [] hv; subst.
+  case: v2=> //=. case: t=> //= i b. case: b=> //= p. by case: p=> //=.
++ move=> v1 v2 t v. rewrite /is_not_comparison /=. case: v1=> //=.
+  + case: v2=> //=. case: t=> //= p. by case: p=> //= [] [] hv; subst.
+  + case: v2=> //= i i'. case: t=> //= p. case: p=> //= sz s. case: s=> //=.
+    + by case: sz=> //= [] [] hv; subst.
+    + by case: sz=> //= [] [] hv; subst.
+    case: v2=> //= b b'. case: t=> //= p. by case: p=> //= [] [] hv; subst.
+  case: v2=> //=. case: t=> //= i b. case: b=> //= p. by case: p=> //=.
++ move=> v1 v2 t v. rewrite /is_not_comparison /=. case: v1=> //=.
+  + case: v2=> //=. case: t=> //= p. by case: p=> //= [] [] hv; subst.
+  + case: v2=> //= i i'. case: t=> //= p. case: p=> //= sz s. case: s=> //=.
+    + by case: sz=> //= [] [] hv; subst.
+    + by case: sz=> //= [] [] hv; subst.
+    case: v2=> //= b b'. case: t=> //= p. case: p=> //= [] [] hv; subst.
+    move: hv. by case: ifP=> //= hb [] hv; subst.
+  case: v2=> //=. case: t=> //= i b. case: b=> //= p. by case: p=> //=.
++ move=> v1 v2 t v. rewrite /is_not_comparison /=. case: v1=> //=.
+  + case: v2=> //=. case: t=> //= p. by case: p=> //= [] [] hv; subst.
+  + case: v2=> //= i i'. case: t=> //= p. case: p=> //= sz s. case: s=> //=.
+    + by case: sz=> //= [] [] hv; subst.
+    + by case: sz=> //= [] [] hv; subst.
+    case: v2=> //= b b'. case: t=> //= p. by case: p=> //= [] [] hv; subst.
+  case: v2=> //=. case: t=> //= i b. case: b=> //= p. by case: p=> //=.
+move=> v1 v2 t v. rewrite /is_not_comparison /=. case: v1=> //=.
++ case: v2=> //=. case: t=> //= p. by case: p=> //= [] [] hv; subst.
++ case: v2=> //= i i'. case: t=> //= p. case: p=> //= sz s. case: s=> //=.
+  + by case: sz=> //= [] [] hv; subst.
+  + by case: sz=> //= [] [] hv; subst.
+  case: v2=> //= b b'. case: t=> //= p. case: p=> //= [] [] hv; subst.
+  move: hv. by case: ifP=> //= hb [] hv; subst.
+case: v2=> //=. case: t=> //= i b. case: b=> //= p. by case: p=> //=.
+Qed.
+
+Lemma sem_binary_operation_val_type1 : forall op v1 v2 t1 t2 v, 
+sem_binary_operation op v1 v2 t1 t2 = Some v ->
+typeof_value v (if (is_not_comparison op) then t1 else (Ptype Tbool)).
+Proof.
+move=> [];rewrite /sem_binary_operation.
++ move=> v1 v2 t1 t2 v /=. case: v1=> //=.
+  + case: v2=> //=. case: t1=> //= p. case: p=> //=.
+    case: t2=> //= p. by case: p=> //=.
+  + case: v2=> //=. case: t1=> //= p i1 i2. case: p=> //= sz s.
+    case: t2=> //= p. by case: p=> //= sz' s' [] hv; subst.
+  + case: v2=> //=. case: t1=> //= p. case: p=> //=.
+    case: t2=> //= p. case: p=> //=.
+  case: v2=> //=. case: t1=> //= i b. case: b=> //= p.
+  case: p=> //= sz s. case: t2=> //= i' b'. case: b'=> //= p.
+  by case: p=> //=.
++ move=> v1 v2 t1 t2 v /=. case: v1=> //=.
+  + case: v2=> //=. case: t1=> //= p. case: p=> //=.
+    case: t2=> //= p. by case: p=> //=.
+  + case: v2=> //=. case: t1=> //= p i1 i2. case: p=> //= sz s.
+    case: t2=> //= p. by case: p=> //= sz' s' [] hv; subst.
+  + case: v2=> //=. case: t1=> //= p. case: p=> //=.
+    case: t2=> //= p. case: p=> //=.
+  + case: v2=> //=. case: t1=> //= i b. case: b=> //= p.
+    case: p=> //= sz s. case: t2=> //= i' b'. case: b'=> //= p.
+    by case: p=> //=.
++ move=> v1 v2 t1 t2 v /=. case: v1=> //=.
+  + case: v2=> //=. case: t1=> //= p. case: p=> //=.
+    case: t2=> //= p. by case: p=> //=.
+  + case: v2=> //=. case: t1=> //= p i1 i2. case: p=> //= sz s.
+    case: t2=> //= p. by case: p=> //= sz' s' [] hv; subst.
+  + case: v2=> //=. case: t1=> //= p. case: p=> //=.
+    case: t2=> //= p. case: p=> //=.
+  + case: v2=> //=. case: t1=> //= i b. case: b=> //= p.
+    case: p=> //= sz s. case: t2=> //= i' b'. case: b'=> //= p.
+    by case: p=> //=.
++ move=> v1 v2 t1 t2 v /=. case: v1=> //=.
+  + case: v2=> //=. case: t1=> //= p. case: p=> //=.
+    case: t2=> //= p. by case: p=> //=.
+  + case: v2=> //=. case: t1=> //= p i1 i2. case: p=> //= sz s.
+    case: t2=> //= p. case: p=> //= sz' s'. case: s=> //=.
+    + case: s'=> //=. case: sz=> //=. case: sz'=> //=. 
+      by case: ifP=> //= ht [] hv; subst.
+    case: s'=> //=. case: sz=> //=. case: sz'=> //=.
+    by case: ifP=> //= hl [] hv; subst.
+  + case: v2=> //=. case: t1=> //= p. case: p=> //=.
+    case: t2=> //= p. case: p=> //=.
+  + case: v2=> //=. case: t1=> //= i b. case: b=> //= p.
+    case: p=> //= sz s. case: t2=> //= i' b'. case: b'=> //= p.
+    by case: p=> //=.
++ move=> v1 v2 t1 t2 v. case: v1=> //=.
+  + case: v2=> //=. case: t1=> //= p.
+    case: p=> //=. case: t2=> //= p. by case: p=> //=.
+  + case: v2=> //=. case: t1=> //= p. case: p=> //= sz s.
+    case: t2=> //= p. by case: p=> //=. 
+  + case: v2=> //= b b'. case: t1=> //= p. case: p=> //=.
+    case: t2=> //= p. by case: p=> //= [] [] hv; subst.
+  case: v2=> //=. case: t1=> //= i b. case: b=> //= p.
+  case: p=> //= sz s. case: t2=> //= i' b'. case: b'=> //= p.
+  by case: p=> //=.
++ move=> v1 v2 t1 t2 v. case: v1=> //=.
+  + case: v2=> //=. case: t1=> //= p.
+    case: p=> //=. case: t2=> //= p. by case: p=> //=.
+  + case: v2=> //=. case: t1=> //= p. case: p=> //= sz s.
+    case: t2=> //= p. by case: p=> //=. 
+  + case: v2=> //= b b'. case: t1=> //= p. case: p=> //=.
+    case: t2=> //= p. by case: p=> //= [] [] hv; subst.
+  case: v2=> //=. case: t1=> //= i b. case: b=> //= p.
+  case: p=> //= sz s. case: t2=> //= i' b'. case: b'=> //= p.
+  by case: p=> //=.
++ move=> v1 v2 t1 t2 v. case: v1=> //=.
+  + case: v2=> //=. case: t1=> //= p.
+    case: p=> //=. case: t2=> //= p. by case: p=> //=.
+  + case: v2=> //=. case: t1=> //= p. case: p=> //= sz s.
+    case: t2=> //= p. by case: p=> //=. 
+  + case: v2=> //= b b'. case: t1=> //= p. case: p=> //=.
+    case: t2=> //= p. by case: p=> //= [] [] hv; subst.
+  case: v2=> //=. case: t1=> //= i b. case: b=> //= p.
+  case: p=> //= sz s. case: t2=> //= i' b'. case: b'=> //= p.
+  by case: p=> //=.
++ move=> v1 v2 t1 t2 v. case: v1=> //=.
+  + case: v2=> //=. case: t1=> //= p.
+    case: p=> //=. case: t2=> //= p. by case: p=> //=.
+  + case: v2=> //=. case: t1=> //= p. case: p=> //= sz s.
+    case: t2=> //= p.  case: p=> //= sz' s' i1 i2.
+    case: sz=> //=. case: sz'=> //=. by case: ifP=> //= hl [] hv; subst.  
+  + case: v2=> //= b b'. case: t1=> //= p. case: p=> //=.
+    case: t2=> //= p. by case: p=> //= [] [] hv; subst.
+  case: v2=> //=. case: t1=> //= i b. case: b=> //= p.
+  case: p=> //= sz s. case: t2=> //= i' b'. case: b'=> //= p.
+  by case: p=> //=.
++ move=> v1 v2 t1 t2 v. case: v1=> //=.
+  + case: v2=> //=. case: t1=> //= p.
+    case: p=> //=. case: t2=> //= p. by case: p=> //=.
+  + case: v2=> //=. case: t1=> //= p. case: p=> //= sz s.
+    case: t2=> //= p.  case: p=> //= sz' s' i1 i2.
+    case: s=> //=.
+    + case: s'=> //=. case: sz=> //=. case: sz'=> //=.
+      case: ifP=> //= hl [] hv; subst.
+   (* case: sz=> //=. case: sz'=> //= by case: ifP=> //= hl [] hv; subst.  
+  + case: v2=> //= b b'. case: t1=> //= p. case: p=> //=.
+    case: t2=> //= p. by case: p=> //= [] [] hv; subst.
+  case: v2=> //=. case: t1=> //= i b. case: b=> //= p.
+  case: p=> //= sz s. case: t2=> //= i' b'. case: b'=> //= p.
+  by case: p=> //=.*)
+Admitted.
+
+Lemma type_reflex : forall v t t' v',
+typeof_value v t ->
+typeof_value v t' ->
+typeof_value v' t ->
+typeof_value v' t'.
+Proof.
+move=> v t t' v'. rewrite /typeof_value /=.
+case: v=> //=.
++ case: t=> //= p. case: p=> //=.
+  case: t'=> //= p'. by case: p'=> //=.
++ case: t=> //= p. case: p=> //=.
+  case: t'=> //= p. by case: p=> //=.
++ case: t=> //= p. case: p=> //=.
+  case: t'=> //= p. by case: p=> //=.
+case: t=> //= i b. case: b=> //= p.
+case: p=> //=. case: t'=> //= i' b. 
+case: b=> //= p. by case: p=> //=.
+Qed.
+
+Lemma eq_type_rel : forall v t t',
+eq_type t t' ->
+typeof_value v t' ->
+typeof_value v t.
+Proof.
+move=> v t t'. case: t'=> //=.
++ case: t=> //= p p'. case: p=> //=.
+  + by case: p'=> //=.
+  + by case: p'=> //=.
+  by case: p'=> //=.
++ case: t=> //= i b i' b'. move=> /andP [] hi.
+  case: b=> //= p. case: b'=> //= p'. case: p=> //=.
+  + by case: p'=> //=.
+  + by case: p'=> //=.
+  case: p'=> //=.
+move=> es e t'. by case: t=> //=.
+Qed.
+  
 (**** Preservation ****)
 Lemma preservation : forall Gamma Sigma genv e ef t st st' v, 
 type_expr Gamma Sigma e ef t ->
 sem_expr genv st e st' v ->
 typeof_value v t.
 Proof.
-(*move=> Gamma Sigma genv e ef t st st' v ht he. move: st st' ef t ht he. elim: e=> //=.
-(* Var *)
+move=> Gamma Sigma genv e ef t st st' v ht he. move: st st' v he.
+induction ht.
 + admit.
-(* Const *)
-+ move=> c t' st st' ef t /= ht /= he; inversion he; subst.
-  (* Int *)
-  + rewrite /typeof_value /=. case: t ht=> //= p.
-    + case: p=> //=.
-      + by move=> ht; inversion ht.
-      + by move=> ht; inversion ht.
-      + by move=> ht; inversion ht.
-    by move=> b ht; inversion ht.
-  by move=> e t ht;inversion ht.
-  (* Bool *)   
-  + rewrite /typeof_value /=. case: t ht=> //= p.
-    + case: p=> //=.
-      + by move=> ht; inversion ht.
-      + by move=> ht; inversion ht.
-      + by move=> ht; inversion ht.
-    by move=> b' ht;inversion ht.
-  by move=> e t ht;inversion ht.
-  (* Unit *)
-  + rewrite /typeof_value /=. case: t ht=> //= p.
-    + case: p=> //=.
-      + by move=> ht; inversion ht.
-      + by move=> ht; inversion ht.
-      + by move=> ht; inversion ht.
-    by move=> b' ht;inversion ht.
-  by move=> e t ht;inversion ht.
-(* App *)
 + admit.
-(* Prim *)
-+ move=> [].
-  (* Ref *)
-  + by move=> es t st st' ef t' ht he;inversion he.
-  (* Deref *)
-  + admit.
-  (* Massgn *)
-  + admit.
-  (* Uop *)
-  + move=> u es t st st' ef t' ht he; inversion ht; subst; inversion he; subst.
-    have hte := type_rel_typeof Gamma Sigma e ef t' H6. rewrite hte in H8. 
-    have := sem_unary_operation_val_type u v0 t' v H8.
++ admit.
++ admit.
++ admit.
++ admit.
+(* Ref *)
++ admit.
+(* Deref *)
++ admit.
+(* Massgn *)
++ admit.
+(* Uop *)
++ move=> st st' v he. inversion he; subst.
+  have [h1 h2] := sem_unary_operation_val_type op v0 (typeof_expr e) v H7.
+  move: (IHht st st' v0 H6)=> hv0t.
+  have := type_rel_typeof Gamma Sigma e ef t ht. case: e ht IHht he H6 H7 h1 h2=> //=.
+  + by move=> v1 ht IHht he H6 H7 h1 h2 <-.
+  + by move=> c t0 ht IHht he H6 H7 h1 h2 <-.
+  + by move=> o e es t0 ht IHht he H6 H7 h1 h2 <-.
+  move=> b es t0 ht IHht he H6 H7 h1 h2. case: b ht IHht he H6=> //=.
+  + by move=> ht IHht he H6 <-.
+  + by move=> ht IHht he H6 <-.
+  + by move=> ht IHht he H6 <-.
+  + by move=> uop ht IHht he H6 <-.
+  + move=> b ht IHht he H6 heq; subst. rewrite heq /= in h2.
+    move: h2. case: ifP=> //= hc hv. + by have := type_reflex v0 t0 t v h1 hv0t hv. 
+    rewrite hc in heq; subst. by have := type_reflex v0 (Ptype Tbool) t v h1 hv0t hv.
+  + by move=> h ht IHht he H6 <-.
+  + by move=> i t0 e e' t1 ht IHht he H6 ho h1 h2 <-.
+  + by move=> e e1 e2 t' ht IHht he H6 ho h1 h2 <-.
+  + by move=> l ht IHht he H6 ho h1 h2 <-.
+  by move=> h e t' ht IHht he H6 ho h1 h2 <-.
+(* Bop *)
++ move=> st st' v he; inversion he; subst.
+  move: (IHht1 st st' v1 H8)=> hvt1.
+  move: (IHht2 st' st'' v2 H9)=> hvt2.
+  move: H. case: ifP=> //= hc.
+  + have ht :=  sem_binary_operation_val_type1 op v1 v2 (typeof_expr e) (typeof_expr e') v H10.
+    move=> heq. have htv1' := eq_type_rel v1 tr t heq hvt1. rewrite hc in ht.
+    have hte := type_rel_typeof Gamma Sigma e ef t ht1.
+    case: e ht1 IHht1 he H8 H10 ht hte=> //=.
+    + move=> vi ht1 IHht1 he H8 H10 ht hte; subst. 
+      by have := eq_type_rel v tr (vtype vi) heq ht. 
+    + move=> c t' ht1 IHht1 he H8 H10 ht hte; subst.
+      by have := eq_type_rel v tr t heq ht. 
+    + move=> i e es t' ht1 IHht1 he H8 H10 ht hte; subst.
+      by have := eq_type_rel v tr t heq ht. 
+    + move=> [] //=.
+      + move=> es t' ht1 IHht1 he H8 H10 ht hte; subst. 
+        by have := eq_type_rel v tr t heq ht. 
+      + move=> es t' ht1 IHht1 he H8 H10 ht hte; subst.
+        by have := eq_type_rel v tr t heq ht. 
+      + move=> es t' ht1 IHht1 he H8 H10 ht hte; subst.
+        by have := eq_type_rel v tr t heq ht. 
+      + move=> uop es t' ht1 IHht1 he H8 H10 ht hte; subst.
+        by have := eq_type_rel v tr t heq ht. 
+      + move=> bop es t' ht1 IHht1 he H8 H10 ht hte; subst. 
+Admitted.
+ 
+
+
+   
+
     
-  *) Admitted.
+    
